src/SoftBound/sb_ds_gv_inject.v
@@ -1866,6 +1866,17 @@ Case "cons".
         apply gv_inject_uninits.
 Qed.
 
+Lemma sb_mem_inj__cgv2gv : forall mi g, 
+  gv_inject mi g g -> gv_inject mi (? g ?) (? g ?).
+Proof.
+  intros.  
+  destruct g; auto.
+  destruct p; auto.
+  destruct v; auto.
+  destruct g; auto.
+  destruct m; apply gv_inject_cons_intro; auto using gv_inject_nil_refl.
+Qed.
+
 Lemma sb_mem_inj__const2GV : forall maxb mi Mem Mem' TD gl c gv,
   wf_sb_mi maxb mi Mem Mem' ->
   wf_globals maxb gl -> 
@@ -1877,7 +1888,8 @@ Proof.
   intros.
   unfold const2GV in H1.
   remember (_const2GV TD gl c) as R.
-  destruct R as [[? ?]|]; inv H1; eauto.
+  destruct R as [[? ?]|]; inv H1; auto.
+  apply sb_mem_inj__cgv2gv; eauto.
 Qed.
 
 Fixpoint gvs_inject mi gvs1 gvs2 : Prop :=
